RelConfig.v
@@ -52,7 +52,8 @@ Inductive wf_val : nat -> L.value -> Prop :=
 | wf_fvar : forall k fvar, wf_val k (var_val (free_var fvar))
 | wf_cst : forall k cst, wf_val k (const_val cst).
 Definition wf_tm (E:local_env) t := trav_tm wf_val (List.length E) t.
-
+Definition wf_func_tm (f:L.function) :=
+  match f with func i t => trav_tm wf_val i t end.
 (* ----------------------------------------------------------
             Local Closure of Lexi terms
    ---------------------------------------------------------- *)
@@ -132,35 +133,45 @@ Definition body t :=
 (* ----------------------------------------------------------
     Initial & Final Predicates for Lexi and Salt 
    ---------------------------------------------------------- *)
-
+Definition ns_hloc : S.word := hloc ""%string 0.
+Definition ns_cloc : S.word := cloc ""%string 0.
+Definition ns_hdl_lab : L.hdl_label := hdl_lab ""%string.
+Definition ns_clab : L.code_label := ""%string.
 Inductive init_S (init_lab main_lab:code_loc): S.program ->
   (S.program * S.heap * reg_file) -> Prop :=
-  mk_init_S : forall (p:program) L_stack,
-  init_S init_lab main_lab
-    p (init_lab !->c
-        ins_seq [mov 0 (cloc main_lab 0); call (reg_o 0);
-          push (reg_o 1); load 1 sp false 0; halt]; p,
-      ((L_stack,stack [])::[],th_empty,(sh_empty, th_empty)),
-         [(ip,loc_w (cloc init_lab 0));(sp,loc_w (hloc L_stack 0));
-          (nat_reg 0,ns);(nat_reg 1,ns);
-          (nat_reg 2,ns);(nat_reg 3,ns);(nat_reg 4,ns);
-          (nat_reg 5,ns);(nat_reg 6,ns)]).
+| mk_init_S : forall (p:program) L_stack dummy_hdl_stk,
+    (* a stack section as a dummy handler *)
+    dummy_hdl_stk = [ns_hloc;int_w 0;ns_hloc;ns_cloc] ->
+    (forall LC x, p = code_trans LC -> wf_func_tm (LC x)) ->
+    init_S init_lab main_lab
+      p (init_lab !->c
+           ins_seq [mov 0 (cloc main_lab 0); call (reg_o 0);
+                    push (reg_o 1); load 1 sp false 0; halt]; p,
+           ([(L_stack,stack dummy_hdl_stk)],th_empty,(sh_empty, th_empty)),
+           [(ip,loc_w (cloc init_lab 0));(sp,loc_w (hloc L_stack 4));
+            (nat_reg 0,ns);(nat_reg 1,ns);
+            (nat_reg 2,ns);(nat_reg 3,ns);(nat_reg 4,ns);
+            (nat_reg 5,ns);(nat_reg 6,ns)]).
 (* note that the value returned after the "exit" doesn't
    matter to the translated program, so we just choose
    000 as an arbitrary value *)
-Inductive init_L (init_lab:code_label): L.program -> (L.code * L.heap *
-  L.eval_context * L.local_env * L.term) -> Prop :=
-  mk_init_L : forall C (H:L.heap) main_lab init_tm,
+Inductive init_L (init_lab:code_label):
+  L.program -> (L.code * L.heap * L.eval_context
+                * L.local_env * L.term) -> Prop :=
+| mk_init_L : forall C (H:L.heap) main_lab init_tm dummy_hdl,
     init_tm = bind (app (c_lab main_lab) [])
-        (bind (exit (var_val 0)) (val_term 000)) ->
+                (bind (exit (var_val 0)) (val_term 000)) ->
+    dummy_hdl = h_f (handler_f ns_hdl_lab
+                       ns_hdl_lab ns_clab general) ->
+    (forall x, wf_func_tm (C x)) ->
     init_L init_lab
       (letrec C init_tm)
-      (init_lab !->c func 0 init_tm ; C, L.h_empty, [] ,[],
-        init_tm)%L_scope.
+      (init_lab !->c func 0 init_tm ; C, L.h_empty, [dummy_hdl] ,[],
+         init_tm)%L_scope.
 Inductive final_L : (L.code * L.heap * L.eval_context *
   L.local_env * L.term) -> nat -> Prop :=
-  mk_final_L : forall C H (i:nat),
-    final_L (C,H,[],[run_const i],L.halt) i.
+  mk_final_L : forall C H K (i:nat),
+    final_L (C,H,K,[run_const i],L.halt) i.
 Inductive final_S : (S.program * S.heap * reg_file) -> word -> Prop :=
   mk_final_S : forall p H_stk H_conts H_tup R (l:code_location)
     (i:nat) lsp S,
@@ -192,7 +203,7 @@ Inductive LS_rel_ins : (L.local_env*L.term) -> S.instr_seq -> Prop :=
 
 Inductive LS_rel_frame : L.a_frame -> S.stack_heap_val -> Prop :=
   rel_frame : forall E t Ilst C_mem C_lab i lst s,
-    LS_rel_ins (E,t) (ins_seq Ilst)
+    LS_rel_ins (L.ns :: E,t) (ins_seq (tl Ilst))
     -> C_mem C_lab = ins_seq (lst ++ Ilst)
     -> List.length lst = i -> LS_rel_env E (stack s) ->
     LS_rel_frame (act_f E t)
@@ -204,59 +215,74 @@ Inductive LS_rel_frames : (list L.frame)
     LS_rel_frame Fi (stack si)
     -> LS_rel_frames Flst (stack s')
     -> LS_rel_frames ((a_f Fi) :: Flst) (stack (si ++ s')).
-Inductive LS_rel_hdl_led_ctx : list L.frame ->
-  (S.word * S.stack_heap_val * S.stack_heap
-  * S.word * S.stack_heap_val) -> Prop :=
-  | rel_hdl_base : forall L s,
-    LS_rel_hdl_led_ctx [] (L,s,sh_empty,L,s)
-  | rel_hdl_general : forall Flst (s s' : list S.word) s_in s_out
-    (L L_env Clab_op L_in:string) L_out  (H_stack:stack_heap) Ks,
+Inductive LS_rel_hdl : L.h_frame -> list S.word -> Prop :=
+| rel_hdl_general : forall (L L_env Clab_op:string) L_prev (s_prev:list word),
+    LS_rel_hdl
+      (handler_f (hdl_lab L)
+              (hdl_lab L_env) Clab_op general)
+      [loc_w (hloc L_prev (List.length s_prev));
+       int_w 0; loc_w (hloc L_env 0);
+       loc_w (c_loc (cloc Clab_op 0))]
+| rel_hdl_other : forall (L L_env Clab_op:string) A num,
+    (A = tail -> num = 1) -> (A = abort -> num = 2) ->
+    LS_rel_hdl
+      (handler_f (hdl_lab L)
+              (hdl_lab L_env) Clab_op A)
+      [ns; int_w num; loc_w (hloc L_env 0);
+       loc_w (c_loc (cloc Clab_op 0))].
+Definition is_general_hdl_frame (f:L.h_frame) : bool :=
+  match f with
+  | handler_f _ _ _ general => true
+  | _ => false
+  end.
+Inductive LS_rel_hdl_stk :
+  list L.frame -> list S.word -> Prop :=
+| rel_hdl_stk_base : forall Flst s frm frm_stk,
     LS_rel_frames Flst (stack s) ->
-    s' = s ++ [loc_w (hloc L_in (List.length s_in));
-      int_w 0; loc_w (hloc L_env 0);
-      loc_w (c_loc (cloc Clab_op 0))]
-    -> LS_rel_hdl_led_ctx Ks 
-       (loc_w (hloc L 0), stack s',H_stack,L_out,s_out) ->
-    LS_rel_hdl_led_ctx
-    ((h_f (handler_f (hdl_lab L)
-      (hdl_lab L_env) Clab_op general)) :: Flst ++ Ks)
-    (loc_w (hloc L_in 0), stack s_in,
-      hloc_str L_in !->s stack s_in ; H_stack,
-      L_out, s_out)
-  | rel_hdl_tail : forall Flst s s' s_in s_out
-    L L_in L_out (L_env Clab_op:string) (H_stack:stack_heap) Ks,
+    LS_rel_hdl frm frm_stk ->
+    is_general_hdl_frame frm = true ->
+    LS_rel_hdl_stk (Flst ++ [h_f frm]) (s ++ frm_stk)
+| rel_hdl_stk : forall Flst s frm frm_stk Klst slst,
+    LS_rel_hdl_stk Klst slst ->
     LS_rel_frames Flst (stack s) ->
-    s' = s ++ [ns; int_w 1; loc_w (hloc L_env 0);
-      loc_w (c_loc (cloc Clab_op 0))] ++ s_in
-    -> LS_rel_hdl_led_ctx Ks 
-       (loc_w (hloc L_in 0), stack s',H_stack,L_out,s_out) ->
-    LS_rel_hdl_led_ctx
-    ((h_f (handler_f (hdl_lab L)
-      (hdl_lab L_env) Clab_op tail)) :: Flst ++ Ks)
-    (loc_w (hloc L_in 0), stack s_in, H_stack, L_out, s_out)
-  | rel_hdl_abort : forall Flst s s' s_in s_out
-    L L_in L_out (L_env Clab_op:string) (H_stack:stack_heap) Ks,
-    LS_rel_frames Flst (stack s) ->
-    s' = s ++ [ns; int_w 2; loc_w (hloc L_env 0);
-      loc_w (c_loc (cloc Clab_op 0))] ++ s_in
-    -> LS_rel_hdl_led_ctx Ks
-       (loc_w (hloc L_in 0), stack s',H_stack,L_out,s_out) ->
-    LS_rel_hdl_led_ctx
-    ((h_f (handler_f (hdl_lab L)
-      (hdl_lab L_env) Clab_op abort)) :: Flst ++ Ks)
-    (loc_w (hloc L_in 0), stack s_in, H_stack, L_out, s_out).
+    LS_rel_hdl frm frm_stk ->
+    is_general_hdl_frame frm = false ->
+    LS_rel_hdl_stk (Flst ++ [h_f frm] ++ Klst) (s ++ frm_stk ++ slst).
+(* ensures that each stack in the list of stacks
+   relates to the corresponding frames of K, in
+   the same and correct order
+   
+   also ensures that all stacks except the first one
+   should point to the previous stack*)
+Inductive LS_rel_hdl_stk_lst :
+  list L.frame -> list (S.heap_loc * S.stack_heap_val) -> Prop :=
+| rel_hdl_stk_nil : LS_rel_hdl_stk_lst [] []
+| rel_hdl_stk_lst : forall Ks H K s L,
+    LS_rel_hdl_stk_lst Ks H ->
+    LS_rel_hdl_stk K s ->
+    LS_rel_hdl_stk_lst (K ++ Ks) ((L,stack s)::H).
+Definition stk_points_to
+  (s s_prev:list S.word) (L:string) :=
+  nth_error (rev s) 3 = Some (loc_w (hloc L (List.length s_prev))).
+(* must have at least 1 stack *)
+Inductive LS_rel_eval_ctx :
+  L.eval_context -> S.stack_heap -> Prop :=
+| rel_hdl_led_ctx : forall Ks H,
+    (forall L s s' L' H',
+        H = [(L,stack s);(hloc_str L',stack s')] ++ H' ->
+        stk_points_to s s' L') ->
+    LS_rel_hdl_stk_lst Ks H ->
+    LS_rel_eval_ctx Ks H.
 
-Inductive LS_rel_context : (L.eval_context * L.local_env) ->
+Inductive LS_rel_env_context : (L.eval_context * L.local_env) ->
   (S.stack_heap * S.heap_location) -> Prop :=
-  rel_context : forall Flst s s' s_out Ks L_0 L_out
-    (E:L.local_env) (H_stack:stack_heap),
-    LS_rel_frames Flst (stack s) ->
-    LS_rel_hdl_led_ctx Ks
-      (loc_w (hloc L_0 0),stack s,H_stack,
-       loc_w (hloc L_out 0),stack s_out) ->
+| rel_env_context :
+  forall s' s_out Ks L_out (E:L.local_env) (H_stack:stack_heap),
+    LS_rel_eval_ctx Ks ((L_out,stack s_out) :: H_stack) ->
     s' = (List.map run_cst_trans E) ++ s_out ->
-    LS_rel_context (Ks ++ Flst, E)
-      ((L_out, stack s') :: H_stack, hloc L_out (List.length s')).
+    LS_rel_env_context (Ks, E)
+      ((L_out, stack s') :: H_stack,
+        hloc L_out (List.length s')).
 Inductive LS_rel_tup_heap : L.tup_heap -> S.tuple_heap -> Prop :=
   rel_tup_heap :
     forall (LH_tup:L.tup_heap) (SH_tup:S.tuple_heap),
@@ -264,39 +290,58 @@ Inductive LS_rel_tup_heap : L.tup_heap -> S.tuple_heap -> Prop :=
         LH_tup (obj_lab L_tup) = L.tuple vs
         -> SH_tup L_tup = tuple (List.map run_cst_trans vs)) ->
     LS_rel_tup_heap LH_tup SH_tup.
+(*
+  
+Inductive LS_rel_cont_stks :
+  list L.frame -> S.stack_heap -> Prop :=
+  rel_cont_stks :
+    LS_rel_hdl_led_ctx Ks H_one_cont ->
+    H_one_cont =
+      [(L_last, stack (s_last))]
+        ++ stks ++
+        [stack (s_0 ++ [loc_w (hloc L_last (List.length s_last));
+                          int_w 0; loc_w (hloc L_env 0);
+                          loc_w (c_loc (cloc Clab_op 0))])]
+                                                          
 Inductive LS_rel_cont_heap :
   L.cont_heap -> (S.stack_heap * S.tuple_heap) -> Prop :=
   rel_cont_heap :
     forall LH_cont SH_cont (SH_ctup:S.tuple_heap),
-      (forall (L_rsp:string) Fs (L:string) L_out L_env  
-           s s_out Ks Clab_op,
-      LH_cont (obj_lab L_rsp) =
-        cont (Ks ++ Fs ++
-                [h_f (handler_f (hdl_lab L) (hdl_lab L_env)
-                        (c_lab Clab_op) general)]) ->
-      LS_rel_frames Fs (stack s) ->
-      LS_rel_hdl_led_ctx Ks
-        (loc_w (hloc L 0),stack s,
-          SH_cont,loc_w (hloc L_out 0), stack s_out) ->
-      SH_ctup L_rsp = tuple [loc_w (hloc L 4)]
-      /\ stk_heap_app SH_cont L_out = stack s_out
-      /\ stk_heap_app SH_cont L =
+      (forall (L_rsp:string) (L:string) L_out L_env  
+              s s_out Ks Clab_op,
+          LH_cont (obj_lab L_rsp) = cont Ks ->
+          Ks = ([h_f (handler_f (hdl_lab L_out) (hdl_lab L_env')
+                        (c_lab Clab_op') general)]
+                  ++ Ks_middle ++
+                  [h_f (handler_f (hdl_lab L) (hdl_lab L_env)
+                          (c_lab Clab_op) general)]) ->
+          LS_rel_hdl_led_ctx Ks SH_cont ->
+          SH_ctup L_rsp = tuple [loc_w (hloc L 4)]
+          /\ stk_heap_app SH_cont L_out = stack s_out
+          /\ stk_heap_app SH_cont L =
            stack (s ++ [loc_w (hloc L_out (List.length s_out));
                         int_w 0;loc_w (hloc L_env 0);loc_w (cloc Clab_op 0)]))
-      -> LS_rel_cont_heap LH_cont (SH_cont,SH_ctup).
+      -> LS_rel_cont_heap LH_cont (SH_cont,SH_ctup).*)
+(* each continuation is a list of stacks, like H_stk.
+   The difference is that the first stack doesn't point
+   back to the context frame where it was cut off, but rather
+   circularly points to the last stack of this continuation.*)
 Inductive LS_rel_heap :
   L.heap -> (S.stack_heap * tuple_heap * tuple_heap) -> Prop :=
   rel_heap :
   forall LH_tup SH_tup
          (SH_conts:stack_heap * tuple_heap) (LH_cont:L.cont_heap),
     LS_rel_tup_heap LH_tup SH_tup ->
-    LS_rel_cont_heap LH_cont SH_conts ->
+    (* LS_rel_cont_heap LH_cont SH_conts -> *)
     LS_rel_heap (LH_tup,LH_cont) (SH_conts,SH_tup).
 Inductive LS_rel_code : L.code -> S.program -> Prop :=
-  | rel_code : forall C, LS_rel_code C (code_trans C)
-  | rel_code_func : forall f (x:string) C,
+| rel_code : forall LC SC,
+    SC = code_trans LC ->
+    (forall x, wf_func_tm (LC x)) ->
+    LS_rel_code LC SC.
+(* | rel_code_func : forall f (x:string) C,
     LS_rel_code (x !->c f ; C)%L_scope
-      (cloc_str x !->c func_trans f; (code_trans C)).
+      (cloc_str x !->c func_trans f; (code_trans C)).*)
 (* A runtime lexi config relates to a runtime salt config if
    subparts of the configs relates to each other accordingly,
    and that the lexi term t is locally closed (i.e. without
@@ -317,7 +362,7 @@ Inductive LS_rel :
     (SH_tup:tuple_heap)
     (Slsp:heap_location) Clab,
     LS_rel_ins (LE,Lt) (ins_seq SIlst) ->
-    LS_rel_context (LK,LE) (SH_stack,Slsp) ->
+    LS_rel_env_context (LK,LE) (SH_stack,Slsp) ->
     LS_rel_heap LH (SH_conts,SH_tup) -> LS_rel_code LC SC ->
     SC Clab = ins_seq (lst ++ SIlst) -> List.length lst = len ->
     (*lc_term Lt \/ body Lt*)
